Pfff, new contraction definition sounds better

src/graph_theory/contraction.lean
@@ -65,6 +65,44 @@ namespace simple_graph
     def is_contraction (G : simple_graph V) (G' : simple_graph V') : Prop
         := ∃ S : contraction.setup G', nonempty (G ≃g (G'/S))
 
+    def is_contraction' (G : simple_graph V) (G' : simple_graph V') : Prop
+        := ∃ φ : V' -> V, surjective φ ∧ G = image φ G'
+
+    example : (∃ S : setoid V', nonempty (G ≃g G'/S)) <-> is_contraction' G G' :=
+    begin
+        split,
+        { rintro ⟨S,⟨⟨f,f',h₁,h₂⟩,h₃⟩⟩,
+            let φ : V' -> V := f' ∘ quotient.mk', refine ⟨φ,_,_⟩,
+            { apply surjective.comp,
+                exact (left_inverse.right_inverse h₁).surjective,
+                exact quotient.surjective_quotient_mk' },
+            { ext a b, rw <-h₃, simp, split,
+                { rintros ⟨p₁,x,y,p₂,p₃,p₄⟩, refine ⟨ne_of_apply_ne f p₁,x,y,_,_,p₄⟩,
+                    have := congr_arg f' p₂, convert this, rw h₁,
+                    have := congr_arg f' p₃, convert this, rw h₁,
+                },
+                { rintros ⟨p₁,x,y,rfl,rfl,p₂⟩, refine ⟨h₁.injective.ne p₁,x,y,_,_,p₂⟩,
+                    simp [φ], rw h₂, refl, simp [φ], rw h₂, refl } }
+        },
+        { rintro ⟨φ,h₁,h₂⟩, subst G,
+            have K := @setoid.ker_apply_mk_out V' V φ,
+            have L := surj_inv_eq h₁,
+            let S : setoid V' := setoid.ker φ, use S,
+            let ψ := (setoid.quotient_ker_equiv_of_surjective φ h₁).symm, refine ⟨⟨ψ,_⟩⟩,
+            introv, split,
+            { rintro ⟨p₁,x,y,p₂,p₃,p₄⟩, refine ⟨ne_of_apply_ne _ p₁,x,y,_,_,p₄⟩,
+                simp [ψ,setoid.quotient_ker_equiv_of_surjective] at p₂,
+                rw [<-K x,p₂], convert K (surj_inv h₁ a), exact (surj_inv_eq h₁ a).symm,
+                simp [ψ,setoid.quotient_ker_equiv_of_surjective] at p₃,
+                rw [<-K y,p₃], convert K (surj_inv h₁ b), exact (surj_inv_eq h₁ b).symm },
+            { rintro ⟨p₁,x,y,rfl,rfl,p₂⟩, refine ⟨ψ.left_inv.injective.ne p₁,x,y,_,_,p₂⟩,
+                simp [ψ,setoid.quotient_ker_equiv_of_surjective], apply quotient.eq.mpr,
+                apply setoid.ker_def.mpr, rw L,
+                simp [ψ,setoid.quotient_ker_equiv_of_surjective], apply quotient.eq.mpr,
+                apply setoid.ker_def.mpr, rw L }
+        }
+    end
+
     infix ` ≼c `:50 := is_contraction
 
     namespace contraction
